src/program_proof/tulip/program/replica/replica_acquire.v
@@ -11,13 +11,9 @@ Section program.
     let ts := uint.nat tsW in
     {{{ own_dbmap_in_slice pwrsS pwrs ∗ own_replica_ptsm_sptsm rp ptsm sptsm }}}
       Replica__acquire #rp #tsW (to_val pwrsS)
-    {{{ (acquired : bool), RET #acquired;
+    {{{ RET #();
         own_dbmap_in_slice pwrsS pwrs ∗
-        if acquired
-        then own_replica_ptsm_sptsm rp (acquire ts pwrs ptsm) (acquire ts pwrs sptsm) ∗
-             ⌜validated_ptsm ptsm pwrs⌝ ∗
-             ⌜validated_sptsm sptsm ts pwrs⌝
-        else own_replica_ptsm_sptsm rp ptsm sptsm
+        own_replica_ptsm_sptsm rp (acquire ts pwrs ptsm) (acquire ts pwrs sptsm)
     }}}.
   Proof.
     iIntros (Hvw ts Φ) "[Hpwrs Hrp] HΦ".
@@ -25,136 +21,16 @@ Section program.
     wp_rec.
     iDestruct (own_replica_ptsm_sptsm_dom with "Hrp") as %[Hdomptsm Hdomsptsm].
 
-    (*@ func (rp *Replica) acquire(ts uint64, pwrs []tulip.WriteEntry) bool {   @*)
-    (*@     // Check if all keys are writable.                                  @*)
-    (*@     var pos uint64 = 0                                                  @*)
-    (*@                                                                         @*)
-    wp_apply (wp_ref_to); first by auto.
-    iIntros (posP) "HposP".
-    wp_pures.
-
-    (*@     for pos < uint64(len(pwrs)) {                                       @*)
-    (*@         ent := pwrs[pos]                                                @*)
-    (*@         writable := rp.writableKey(ts, ent.Key)                         @*)
-    (*@         if !writable {                                                  @*)
-    (*@             break                                                       @*)
-    (*@         }                                                               @*)
-    (*@         pos++                                                           @*)
-    (*@     }                                                                   @*)
-    (*@                                                                         @*)
-    iDestruct (own_slice_sz with "HpwrsS") as %Hlen.
-    iDestruct (own_slice_small_acc with "HpwrsS") as "[HpwrsS HpwrsC]".
-    set P := (λ (cont : bool), ∃ (pos : u64),
-      let pwrs' := list_to_map (take (uint.nat pos) pwrsL) in
-      "HpwrsS"  ∷ own_slice_small pwrsS (struct.t WriteEntry) (DfracOwn 1) pwrsL ∗
-      "HposP"   ∷ posP ↦[uint64T] #pos ∗
-      "Hrp"     ∷ own_replica_ptsm_sptsm rp ptsm sptsm ∗
-      "%Hptsm"  ∷ ⌜validated_ptsm ptsm pwrs'⌝ ∗
-      "%Hsptsm" ∷ ⌜validated_sptsm sptsm ts pwrs'⌝)%I.
-    wp_apply (wp_forBreak_cond P with "[] [HpwrsS HposP Hrp]"); last first; first 1 last.
-    { (* Loop entry. *)
-      iExists (W64 0).
-      rewrite uint_nat_W64_0 take_0 list_to_map_nil.
-      iFrame.
-      iPureIntro.
-      (* split; first done. *)
-      split.
-      { rewrite /validated_ptsm dom_empty_L.
-        intros k n Hn.
-        by apply map_lookup_filter_Some in Hn as [_ ?].
-      }
-      { rewrite /validated_sptsm dom_empty_L.
-        intros k n Hn.
-        by apply map_lookup_filter_Some in Hn as [_ ?].
-      }
-    }
-    { (* Loop body. *)
-      clear Φ. iIntros (Φ) "!> HP HΦ". iNamed "HP".
-      wp_load.
-      wp_apply (wp_slice_len).
-      wp_if_destruct; last first.
-      { (* Exit from the loop condition. *)
-        iApply "HΦ".
-        iExists pos.
-        by iFrame "∗ %".
-      }
-      wp_load.
-      destruct (lookup_lt_is_Some_2 pwrsL (uint.nat pos)) as [[k v] Hwr]; first word.
-      wp_apply (wp_SliceGet with "[$HpwrsS]"); first done.
-      iIntros "HpwrsL".
-      wp_pures.
-      wp_apply (wp_Replica__writableKey with "Hrp").
-      { apply elem_of_list_lookup_2 in Hwr.
-        rewrite -HpwrsL in Hwr.
-        apply elem_of_map_to_list, elem_of_dom_2 in Hwr.
-        clear -Hvw Hwr. set_solver.
-      }
-      iIntros (ok) "[Hrp %Hwritable]".
-      wp_pures.
-      destruct ok; wp_pures; last first.
-      { iApply "HΦ".
-        by iFrame "∗ %".
-      }
-      wp_load.
-      wp_store.
-      iApply "HΦ".
-      iFrame "∗ %".
-      iPureIntro.
-      rewrite uint_nat_word_add_S; last word.
-      rewrite (take_S_r _ _ _ Hwr) list_to_map_snoc; last first.
-      { by eapply map_to_list_not_elem_of_take_key. }
-      split.
-      { intros x n Hn.
-        apply map_lookup_filter_Some in Hn as [Hn Hx].
-        rewrite /= dom_insert_L elem_of_union in Hx.
-        destruct Hx as [Hx | Hx]; last first.
-        { specialize (Hptsm x n). simpl in Hptsm.
-          apply Hptsm.
-          by apply map_lookup_filter_Some.
-        }
-        rewrite elem_of_singleton in Hx. subst x.
-        destruct Hwritable as [Hwritable _].
-        by rewrite /key_writable_ptsm Hn in Hwritable.
-      }
-      { intros x n Hn.
-        apply map_lookup_filter_Some in Hn as [Hn Hx].
-        rewrite /= dom_insert_L elem_of_union in Hx.
-        destruct Hx as [Hx | Hx]; last first.
-        { specialize (Hsptsm x n). simpl in Hsptsm.
-          apply Hsptsm.
-          by apply map_lookup_filter_Some.
-        }
-        rewrite elem_of_singleton in Hx. subst x.
-        destruct Hwritable as [_ Hwritable].
-        by rewrite /key_writable_sptsm Hn in Hwritable.
-      }
-    }
-    iNamed 1. clear P.
-
-    (*@     // Report error if some key cannot be locked.                       @*)
-    (*@     if pos < uint64(len(pwrs)) {                                        @*)
-    (*@         return false                                                    @*)
-    (*@     }                                                                   @*)
-    (*@                                                                         @*)
-    wp_load.
-    wp_apply wp_slice_len.
-    wp_if_destruct.
-    { iDestruct ("HpwrsC" with "HpwrsS") as "HpwrsS".
-      iApply "HΦ".
-      by iFrame "∗ %".
-    }
-    rewrite take_ge in Hptsm, Hsptsm; last word.
-    pose proof (list_to_map_flip _ _ HpwrsL) as Hltm.
-    rewrite -Hltm in Hptsm, Hsptsm.
-
-    (*@     // Acquire locks for each key.                                      @*)
+    (*@ func (rp *Replica) acquire(ts uint64, pwrs []tulip.WriteEntry) {        @*)
     (*@     for _, ent := range(pwrs) {                                         @*)
     (*@         rp.acquireKey(ts, ent.Key)                                      @*)
     (*@     }                                                                   @*)
-    (*@                                                                         @*)
+    (*@ }                                                                       @*)
+    iDestruct (own_slice_sz with "HpwrsS") as %Hlen.
+    iDestruct (own_slice_small_acc with "HpwrsS") as "[HpwrsS HpwrsC]".
     set P := (λ (i : u64),
-      let pwrs' := list_to_map (take (uint.nat i) pwrsL) in
-      own_replica_ptsm_sptsm rp (acquire ts pwrs' ptsm) (acquire ts pwrs' sptsm))%I.
+                let pwrs' := list_to_map (take (uint.nat i) pwrsL) in
+                own_replica_ptsm_sptsm rp (acquire ts pwrs' ptsm) (acquire ts pwrs' sptsm))%I.
     wp_apply (wp_forSlice P with "[] [$HpwrsS Hrp]"); last first; first 1 last.
     { (* Loop entry. *)
       subst P. simpl.
@@ -187,13 +63,11 @@ Section program.
       done.
     }
     iIntros "[HP HpwrsS]".
-    iNamed "HP". clear P.
-    rewrite -Hlen firstn_all -Hltm in Hptsmabs, Hsptsmabs.
-
-    (*@     return true                                                         @*)
-    (*@ }                                                                       @*)
-    wp_pures.
     iDestruct ("HpwrsC" with "HpwrsS") as "HpwrsS".
+    iNamed "HP". clear P.
+    pose proof (list_to_map_flip _ _ HpwrsL) as Hltm.
+    rewrite -Hlen firstn_all -Hltm in Hptsmabs, Hsptsmabs.
+    wp_pures.
     iApply "HΦ".
     by iFrame "HptsmP HsptsmP ∗ %".
   Qed.
