src/program_proof/tulip/program/replica/replica_memorize.v
@@ -1,0 +1,34 @@
+From Perennial.program_proof.tulip.program Require Import prelude replica_repr.
+
+Section program.
+  Context `{!heapGS Σ, !tulip_ghostG Σ}.
+
+  Theorem wp_Replica__memorize
+    rp (tsW : u64) pwrsS pwrs (ptgsS : Slice.t) (cpm : gmap nat dbmap) :
+    let ts := uint.nat tsW in
+    {{{ own_dbmap_in_slice pwrsS pwrs ∗ own_replica_cpm rp cpm }}}
+      Replica__memorize #rp #tsW (to_val pwrsS) (to_val ptgsS)
+    {{{ RET #(); own_replica_cpm rp (<[ts := pwrs]> cpm) }}}.
+  Proof.
+    iIntros (ts Φ) "[Hpwrs Hcpm] HΦ".
+    wp_rec.
+
+    (*@ func (rp *Replica) memorize(ts uint64, pwrs []tulip.WriteEntry, ptgs []uint64) { @*)
+    (*@     rp.prepm[ts] = pwrs                                                 @*)
+    (*@     // rp.ptgsm[ts] = ptgs                                              @*)
+    (*@ }                                                                       @*)
+    iNamed "Hcpm".
+    wp_loadField.
+    wp_apply (wp_MapInsert with "HprepmS"); first done.
+    iIntros "HprepmS".
+    wp_pures.
+    iApply "HΦ".
+    iDestruct (big_sepM2_insert_2 _ _ _ tsW with "[Hpwrs] Hprepm") as "Hprepm".
+    { iFrame "Hpwrs". }
+    iFrame.
+    iPureIntro.
+    rewrite 2!kmap_insert.
+    f_equal; [word | done].
+  Qed.
+
+End program.
